improved section cohesion

src/Rdf.v
@@ -73,8 +73,8 @@ Section Rdf.
       (ts : seq (triple I B1 L)) : seq (triple I B2 L) :=
       map (relabeling_triple mu) ts.
 
-    Section Relabeling_seq_triple.
-      Variable B1 : Type.
+    Section Relabeling_seq_triple_poly.
+      Variable B1 B2 B3 : Type.
 
       Lemma relabeling_seq_triple_id ts : relabeling_seq_triple id ts = ts.
       Proof. by elim ts => [//| t ts' ihts] /=; rewrite relabeling_triple_id ihts. Qed.
@@ -83,50 +83,94 @@ Section Rdf.
         mu1 =1 mu2 -> relabeling_seq_triple mu1 ts = relabeling_seq_triple mu2 ts.
       Proof. move=> mu_eq; apply: eq_map; exact: relabeling_triple_ext. Qed.
 
-      Lemma relabeling_seq_triple_comp (B2 : eqType) (mu2 : B -> B1) (mu1 : B1 -> B2) ts :
+      Lemma relabeling_seq_triple_comp (mu2 : B1 -> B2) (mu1 : B2 -> B3) (ts : seq (triple I B1 L)) :
         relabeling_seq_triple mu1 (relabeling_seq_triple mu2 ts) =
           relabeling_seq_triple (mu1 \o mu2) ts.
       Proof.
         by rewrite /relabeling_seq_triple -map_comp; apply: eq_map=> x; rewrite relabeling_triple_comp.
       Qed.
 
-      Lemma relabeling_seq_triple_nil (B2 : Type) (mu : B1 -> B2) :
+      Lemma relabeling_triple_map_comp (ts : seq (triple I B1 L)) (mu1: B1 -> B2) (mu2 : B2 -> B3) :
+        [seq relabeling_triple mu2 i | i <- [seq relabeling_triple mu1 i | i <- ts]] =
+          [seq relabeling_triple (mu2 \o mu1) i | i <- ts].
+      Proof. have ->: [seq relabeling_triple (mu2 \o mu1) i | i <- ts] = relabeling_seq_triple (mu2 \o mu1) ts by [].
+             by rewrite -relabeling_seq_triple_comp.
+      Qed.
+
+      Lemma relabeling_seq_triple_nil (mu : B1 -> B2) :
         relabeling_seq_triple mu [::] = [::].
       Proof. by []. Qed.
 
-    End Relabeling_seq_triple.
+      Lemma eq_relabeling_seq_triple (mu nu : B1 -> B2) : mu =1 nu -> (relabeling_seq_triple mu) =1 (relabeling_seq_triple nu).
+      Proof. by move=> feq; elim=> [//| h t IHtl]; rewrite /= (eq_relabeling_triple feq) IHtl. Qed.
+
+
+    End Relabeling_seq_triple_poly.
+    Section Relabeling_seq_triple_eq.
+
+      Lemma uniq_rdf_graph g : uniq g. Proof. exact: ugraph. Qed.
+      Hint Resolve uniq_rdf_graph.
+
+      Lemma bijective_perm_eq_relabeling_st mu nu ts1 ts2 :
+      uniq (relabeling_seq_triple nu ts1) ->
+      cancel mu nu -> perm_eq (relabeling_seq_triple mu ts2) ts1 -> perm_eq ts2 (relabeling_seq_triple nu ts1).
+      Proof. move=> urtnu can_munu /(perm_map (relabeling_triple nu)) peq.
+             have can_id: {in ts2, [eta relabeling_triple (nu \o mu)] =1 id}.
+             by move=>  [[]s []p []o ? ?] _ //; apply triple_inj=> //=; rewrite can_munu.
+             have peq_can: perm_eq ts2 [seq relabeling_triple nu i | i <- relabeling_seq_triple mu ts2].
+             by rewrite relabeling_triple_map_comp map_id_in //.
+             apply: perm_trans peq_can peq.
+      Qed.
+
+      Lemma perm_eq_relab_uniq g1 g2 mu : perm_eq (relabeling_seq_triple mu g1) g2 -> perm_eq (relabeling_seq_triple mu g1) g2 /\ uniq (relabeling_seq_triple mu g1).
+      Proof. by move=> peq; rewrite (perm_uniq peq) peq. Qed.
+
+
+      Lemma relabeling_triple_comp_map (B1 B2 B3 : eqType) (g : rdf_graph I B1 L) (mu12 : B1 -> B2) (mu23 : B2 -> B3) :
+        [seq relabeling_triple mu23 i | i <- relabeling_seq_triple mu12 g] =
+          relabeling_seq_triple (mu23 \o mu12) g.
+      Proof. case g=> g' us=> /=; rewrite -map_comp.
+             by elim g'=> [//| h t IHts] /=; last by rewrite relabeling_triple_comp -IHts.
+      Qed.
+
+      Lemma perm_eq_comp ts1 ts2 ts3 mu12 mu23:
+        perm_eq (relabeling_seq_triple mu12 ts1) ts2 ->
+        perm_eq (relabeling_seq_triple mu23 ts2) ts3 ->
+        perm_eq (relabeling_seq_triple (mu23 \o mu12) ts1) ts3.
+      Proof. by move=> /(perm_map (relabeling_triple mu23)); rewrite relabeling_triple_map_comp; apply perm_trans. Qed.
+
+    End Relabeling_seq_triple_eq.
+
+    (* End Relabeling_seq_triple. *)
+
+    Section Rdf_mem.
+
+      Lemma rdf_perm_mem_eq {i b l : eqType} (g1 g2 :rdf_graph i b l) :
+        (perm_eq g1 g2) <-> (g1 =i g2).
+      Proof. split; first by move=> /perm_mem.
+             by move: (ugraph g1) (ugraph g2); apply uniq_perm.
+      Qed.
+
+      Lemma rdf_mem_eq_graph g1 g2 :
+        g1 =i g2 <-> (graph g1) =i (graph g2).
+      Proof. by []. Qed.
+
+    End Rdf_mem.
 
     Definition relabeling
       (B1 B2 : eqType) (mu : B1 -> B2)
       (g : rdf_graph I B1 L)  (urel : uniq (relabeling_seq_triple mu (graph g))): rdf_graph I B2 L:=
       mkRdfGraph urel.
 
-    Lemma relabeling_triple_map_comp (B1 B2: eqType) (ts : seq (triple I B L)) (mu1: B -> B1) (mu2 : B1 -> B2) :
-      [seq relabeling_triple mu2 i | i <- [seq relabeling_triple mu1 i | i <- ts]] =
-        [seq relabeling_triple (mu2 \o mu1) i | i <- ts].
-    Proof. have ->: [seq relabeling_triple (mu2 \o mu1) i | i <- ts] = relabeling_seq_triple (mu2 \o mu1) ts by [].
-           by rewrite -relabeling_seq_triple_comp.
-    Qed.
-
-    Lemma rdf_perm_mem_eq {i b l : eqType} (g1 g2 :rdf_graph i b l) :
-      (perm_eq g1 g2) <-> (g1 =i g2).
-    Proof. split; first by move=> /perm_mem.
-           by move: (ugraph g1) (ugraph g2); apply uniq_perm.
-    Qed.
-
-    Lemma rdf_mem_eq_graph g1 g2 :
-      g1 =i g2 <-> (graph g1) =i (graph g2).
-    Proof. by []. Qed.
-
-    Lemma relabeling_comp (B1 B2: eqType) g (mu1 : B -> B1) (mu2: B1 -> B2) :
-      forall u1 u2 u12,
-        perm_eq (@relabeling B1 B2 mu2 (@relabeling B B1 mu1 g u1) u2) (@relabeling B B2 (mu2 \o mu1) g u12).
-    Proof. move=> u1 u2 u12; rewrite rdf_perm_mem_eq /relabeling/==> x /=.
-           suffices ->: {| graph := relabeling_seq_triple mu2 (relabeling_seq_triple mu1 g); ugraph := u2 |} = {| graph := relabeling_seq_triple (mu2 \o mu1) g; ugraph := u12 |} by [].
-           by apply rdf_inj; rewrite /= relabeling_seq_triple_comp.
-    Qed.
-
     Section Relabeling_graph.
+
+      Lemma relabeling_comp (B1 B2: eqType) g (mu1 : B -> B1) (mu2: B1 -> B2) :
+        forall u1 u2 u12,
+          perm_eq (@relabeling B1 B2 mu2 (@relabeling B B1 mu1 g u1) u2) (@relabeling B B2 (mu2 \o mu1) g u12).
+      Proof. move=> u1 u2 u12; rewrite rdf_perm_mem_eq /relabeling/==> x /=.
+             suffices ->: {| graph := relabeling_seq_triple mu2 (relabeling_seq_triple mu1 g); ugraph := u2 |} = {| graph := relabeling_seq_triple (mu2 \o mu1) g; ugraph := u12 |} by [].
+             by apply rdf_inj; rewrite /= relabeling_seq_triple_comp.
+      Qed.
 
       Lemma relabeling_id g : forall us, (@relabeling B B id g us) = g.
       Proof. by case g => g' ug us ; apply rdf_inj=> /=; rewrite relabeling_seq_triple_id. Qed.
@@ -147,81 +191,312 @@ Section Rdf.
             mkRdfGraph (undup_uniq (relabeling_triple mu trpl :: (relabeling_seq_triple mu ts))).
       Proof. by move=> us; apply rdf_inj=> /=; move: us=> /andP[/negPf -> /undup_id ->]. Qed.
 
+      Lemma bijective_eqb_rdf mu nu g1 g2 :
+        forall us1 us2,
+          cancel mu nu -> eqb_rdf (@relabeling _ _ mu g2 us1) g1 -> eqb_rdf g2 (@relabeling _ _ nu g1 us2).
+      Proof.
+        by move=> us1 us2 can_munu; rewrite /eqb_rdf/relabeling/=; apply bijective_perm_eq_relabeling_st.
+      Qed.
+
+      Lemma eqb_relabeling_comp g1 g2 g3 mu12 mu23:
+        forall u1 u2 u3,
+          eqb_rdf (@relabeling _ _ mu12 g1 u1) g2 ->
+          eqb_rdf (@relabeling _ _ mu23 g2 u2) g3 ->
+          eqb_rdf (@relabeling _ _ (mu23 \o mu12) g1 u3) g3.
+      Proof. by move=> u1 u2 u3; apply perm_eq_comp. Qed.
+
+
     End Relabeling_graph.
 
-    Definition terms_ts {i b l : eqType} (ts : seq (triple i b l)) : seq (term i b l) :=
-      undup (flatten (map (@terms_triple i b l) ts)).
+    Section Terms_ts.
 
-    Lemma undup_terms_ts ts : undup (terms_ts ts) = (terms_ts ts).
-    Proof. by rewrite undup_idem. Qed.
+      Definition terms_ts {i b l : eqType} (ts : seq (triple i b l)) : seq (term i b l) :=
+        undup (flatten (map (@terms_triple i b l) ts)).
 
-    Lemma uniq_terms_ts (i b l : eqType) (ts : seq (triple i b l)) : uniq (terms_ts ts).
-    Proof. by apply undup_uniq. Qed.
-    Hint Resolve uniq_terms_ts.
+      Lemma undup_terms_ts ts : undup (terms_ts ts) = (terms_ts ts).
+      Proof. by rewrite undup_idem. Qed.
 
-    Remark uniq_tail (T: eqType) a (t : seq T) : (uniq (a :: t)) -> uniq t.
-    Proof. by move=> /andP[_ //]. Qed.
+      Lemma uniq_terms_ts (i b l : eqType) (ts : seq (triple i b l)) : uniq (terms_ts ts).
+      Proof. by apply undup_uniq. Qed.
+      Hint Resolve uniq_terms_ts.
 
-    Lemma terms_ts_cons {i b l : eqType} (trpl : triple i b l) (ts : seq (triple i b l)) :
-      terms_ts (trpl :: ts) = undup (terms_triple trpl ++ (terms_ts ts)).
-    Proof. by case: ts =>  [ // | ? ? /= ]; rewrite undup_cat_r. Qed.
+      Remark uniq_tail (T: eqType) a (t : seq T) : (uniq (a :: t)) -> uniq t.
+      Proof. by move=> /andP[_ //]. Qed.
 
-    Definition terms {i b l : eqType} (g : rdf_graph i b l) : seq (term i b l) :=
-      undup (flatten (map (@terms_triple i b l) (graph g))).
+      Lemma terms_ts_cons {i b l : eqType} (trpl : triple i b l) (ts : seq (triple i b l)) :
+        terms_ts (trpl :: ts) = undup (terms_triple trpl ++ (terms_ts ts)).
+      Proof. by case: ts =>  [ // | ? ? /= ]; rewrite undup_cat_r. Qed.
 
-    Lemma terms_graph {i b l: eqType} (g : rdf_graph i b l) :
-      terms g = terms_ts (graph g).
-    Proof. by case g. Qed.
+      Lemma mem_triple_terms_ts t ts: t \in ts -> [&& (subject t) \in (terms_ts ts),
+              ((predicate t) \in (terms_ts ts)) & ((object t) \in terms_ts ts)].
+      Proof. case t=> s p o ? ? /=; elim: ts=> [//|hd tl IHts] /= t_mem.
+             apply /and3P; rewrite !terms_ts_cons !mem_undup; move: t_mem; rewrite !in_cons /terms_triple !mem_cat; case/orP.
+             + by move=> /eqP <-; rewrite !mem_undup !in_cons !eqxx /= !orbT.
+             + by move=> /IHts /and3P[-> -> ->]; rewrite !orbT.
+      Qed.
 
-    Lemma undup_terms g : undup (terms g) = (terms g).
-    Proof. by rewrite terms_graph undup_terms_ts. Qed.
+      Section Term_ts_Relabeling.
+        Variable B1 B2: eqType.
 
-    Lemma uniq_terms {i b l : eqType} (g : rdf_graph i b l) : uniq (terms g).
-    Proof. by apply undup_uniq. Qed.
-    Hint Resolve uniq_terms.
+        Lemma terms_ts_relabeled_mem (ts : seq (triple I B1 L)) (mu: B1 -> B2) :
+        (terms_ts (relabeling_seq_triple mu ts)) =i (map (relabeling_term mu) (terms_ts ts)).
+        Proof. elim: ts=> [//| h t IHt] /= x.
+               by rewrite !terms_ts_cons !mem_undup -mem_map_undup map_cat !mem_cat IHt terms_relabeled_triple_mem.
+        Qed.
 
-    Lemma terms_cons {i b l : eqType} (trpl : triple i b l) (ts : seq (triple i b l)) (us : uniq (trpl :: ts)):
-      terms (mkRdfGraph us) = undup (terms_triple trpl ++ (terms (mkRdfGraph (uniq_tail us)))).
-    Proof. by rewrite !terms_graph terms_ts_cons. Qed.
+        Lemma terms_ts_relabeled (ts : seq (triple I B1 L)) (mu : B1 -> B2) (mu_inj: injective mu):
+          terms_ts (relabeling_seq_triple mu ts) = [seq relabeling_term mu i | i <- terms_ts ts].
+        Proof.
+          have /(_ I L) rts_inj := (relabeling_triple_inj mu_inj).
+          have /(_ I L) rt_inj := (relabeling_term_inj mu_inj).
+          elim: ts=> [//| h tl IHtl].
+          have step: undup ([seq relabeling_term mu i | i <- terms_triple h] ++
+                            [seq relabeling_term mu i | i <- flatten [seq terms_triple i | i <- tl]]) =
+                 undup
+                   ([seq relabeling_term mu i | i <- terms_triple h] ++
+                      undup [seq relabeling_term mu i | i <- flatten [seq terms_triple i | i <- tl]]) by rewrite undup_cat_r.
+          rewrite -undup_map_inj // !terms_ts_cons /= map_cat step.
+          by apply f_equal; rewrite IHtl terms_relabeled_triple // undup_map_inj.
+        Qed.
+
+      End Term_ts_Relabeling.
+
+      Section Bnodes_ts.
+        Definition bnodes_ts (i b l : eqType) (ts : seq (triple i b l)): seq (term i b l) :=
+        undup (filter (@is_bnode i b l) (terms_ts ts)).
+
+        Lemma bnodes_ts_cons (trpl : triple I B L) (ts : seq (triple I B L)) :
+          bnodes_ts (trpl :: ts) = undup ((bnodes_triple trpl) ++ (bnodes_ts ts)).
+        Proof. by rewrite /bnodes_ts terms_ts_cons filter_undup undup_idem undup_cat_r filter_cat. Qed.
+
+        Lemma all_bnodes_ts ts : all (@is_bnode I B L) (bnodes_ts ts).
+        Proof. elim: ts=> [// | t ts IHts].
+               by rewrite bnodes_ts_cons all_undup all_cat IHts Bool.andb_true_r all_bnodes_triple_is_bnode.
+        Qed.
+
+        Lemma all_bnodes_perm ts s:
+          perm_eq (bnodes_ts ts) s -> forall x, x \in s -> is_bnode x.
+        Proof. by move=> peq x xin; apply (in_all xin); rewrite -(perm_all _ peq) all_bnodes_ts. Qed.
+
+        Lemma uniq_bnodes_ts ts : uniq (bnodes_ts ts).
+        Proof. exact: undup_uniq. Qed.
+        Hint Resolve uniq_bnodes_ts.
+
+        Lemma i_in_bnodes_ts id ts: Iri id \in bnodes_ts ts = false.
+        Proof. by rewrite /bnodes_ts -filter_undup mem_filter. Qed.
+
+        Lemma l_in_bnodes_ts l ts: Lit l \in bnodes_ts ts = false.
+        Proof. by rewrite /bnodes_ts -filter_undup mem_filter. Qed.
+
+      Lemma bterms_ts b ts : Bnode b \in (terms_ts ts) -> Bnode b \in (bnodes_ts ts).
+      Proof. by move=> mem_term; rewrite mem_undup mem_filter. Qed.
+
+        Section Bnodes_ts_relabeling.
+          Variables B1 B2 : eqType.
+
+          Lemma filter_map_rt (trms: seq (term I B1 L)) (us: uniq trms) (mu: B1 -> B2) :
+            [seq x <- [seq relabeling_term mu i | i <- trms ] | is_bnode x] =i
+                                                                             [seq relabeling_term mu i | i <- trms & is_bnode i].
+          Proof. elim: trms us=> [//| hd tl IHtl] [/andP[nin utl]] x /=.
+                 case e: (is_bnode hd) nin.
+                 by rewrite bnodes_to_bnodes //= in_cons IHtl.
+                 have -> : is_bnode (relabeling_term mu hd) = false by move : e; case hd=> //.
+                 by rewrite IHtl.
+          Qed.
+
+          Lemma bnodes_ts_relabel_mem (ts : seq (triple I B1 L)) (mu: B1 -> B2) :
+            bnodes_ts (relabeling_seq_triple mu ts) =i (map (relabeling_term mu) (bnodes_ts ts)).
+          Proof. move=> x; rewrite mem_undup -mem_map_undup.
+                 by rewrite mem_filter terms_ts_relabeled_mem -mem_filter filter_map_rt.
+          Qed.
+
+          Lemma bnodes_ts_relabel_inj (ts: seq (triple I B1 L)) (mu: B1 -> B2) (mu_inj : injective mu):
+            bnodes_ts (relabeling_seq_triple mu ts) = (map (relabeling_term mu) (bnodes_ts ts)).
+          Proof.
+            have /(_ I L) rtmu_inj := relabeling_term_inj mu_inj.
+            rewrite /bnodes_ts terms_ts_relabeled // -filter_undup undup_map_inj // -filter_undup.
+            elim: (undup (terms_ts ts)) => [// | hd tl IHtl] /=.
+                 case e: (is_bnode hd).
+                 by rewrite bnodes_to_bnodes // IHtl.
+                 have -> : is_bnode (relabeling_term mu hd) = false by move : e; case hd=> //.
+                 by rewrite IHtl.
+          Qed.
+
+          Lemma bnodes_map_get_bs ts : bnodes_ts ts = map (fun b=> Bnode b) (get_bs (bnodes_ts ts)).
+          Proof.
+            move: (all_bnodes_ts ts).
+            rewrite /bnodes_ts filter_undup // undup_idem -filter_undup.
+            elim: [seq x <- undup (flatten [seq terms_triple i | i <- ts]) | is_bnode x]=> [//| []//=b t IHt] al.
+            by rewrite -IHt.
+          Qed.
+
+          Lemma bterm_eq_mem_get_bs (b: B) ts :
+            (@Bnode I B L b) \in terms_ts ts ->
+                                 b \in get_bs (bnodes_ts ts).
+          Proof. by move=> /bterms_ts; rewrite {1}bnodes_map_get_bs (mem_map  (@bnode_inj I B L)). Qed.
+
+          (* TODO split lemma *)
+          Lemma mem_ts_mem_triple_bs t ts b : t \in ts -> Bnode b \in bnodes_triple t -> b \in get_bs (bnodes_ts ts).
+          Proof. move=> /mem_triple_terms_ts; case t=> [[]]s []p []o ? ? //= /and3P[sint pint oint];
+                                                  rewrite /bnodes_triple filter_undup mem_undup ?in_cons in_nil // Bool.orb_false_r=> /eqP[eq]; move: sint oint; rewrite ?eq=> sint oint; rewrite bterm_eq_mem_get_bs //.
+                 by move: eq=> /eqP; case/orP=> /eqP[->].
+          Qed.
+
+          Lemma can_bs_can_rtbs ts (mu nu: B -> B) : {in get_bs (bnodes_ts ts), nu \o mu =1 id} ->
+                                                 {in ts, [eta relabeling_triple (nu \o mu)] =1 id}.
+          Proof. move=> /= in_getb [s p o sib pii] /mem_ts_mem_triple_bs ing /=; apply triple_inj=> /=.
+                 + case: s sib ing  => // b sib ing.
+                   by rewrite /= in_getb // ing // /bnodes_triple filter_undup mem_undup in_cons eqxx.
+                 + by case: p pii ing  => // b sib /mem_g_mem_triple_b inb /=.
+                 + case: o ing  => // b ing /=.
+                   by rewrite /= in_getb // ing // /bnodes_triple filter_undup mem_undup mem_filter -mem_rev in_cons eqxx.
+          Qed.
+
+        End Bnodes_ts_relabeling.
+
+        Definition get_bts {i b l : eqType} (ts : seq (triple i b l)) : seq b :=
+          get_bs (bnodes_ts ts).
+
+        Lemma mem_ts_mem_triple_bts t ts b : t \in ts -> Bnode b \in bnodes_triple t -> b \in get_bts ts.
+        Proof. by apply mem_ts_mem_triple_bs. Qed.
+
+        Lemma bnodes_map_get_bts ts : bnodes_ts ts = map (fun b=> Bnode b) (get_bts ts).
+        Proof. exact: bnodes_map_get_bs. Qed.
+
+        Lemma uniq_get_bs ts : uniq (get_bs (bnodes_ts ts)).
+        Proof. by rewrite -(undup_get_bsC (uniq_bnodes_ts ts)) undup_uniq. Qed.
+        Hint Resolve uniq_get_bs.
+
+        Lemma uniq_get_bts ts : uniq (get_bts ts).
+        Proof. by rewrite uniq_get_bs. Qed.
+
+        Lemma bterm_eq_mem_get_bts (b: B) ts :
+          (@Bnode I B L b) \in terms_ts ts ->
+                               b \in get_bs (bnodes_ts ts).
+        Proof. by apply bterm_eq_mem_get_bs. Qed.
+
+        Lemma perm_relabel_bnodes_ts ts1 ts2 mu :
+          perm_eq [seq relabeling_term mu i | i <- bnodes_ts ts1] (bnodes_ts ts2) =
+            perm_eq [seq mu i | i <- get_bs (bnodes_ts ts1)] (get_bs (bnodes_ts ts2)).
+        Proof. rewrite -(get_bs_map mu (all_bnodes_ts ts1)).
+               case e : (perm_eq [seq relabeling_term mu i | i <- bnodes_ts ts1] (bnodes_ts ts2)).
+               +  have urt_l : uniq [seq relabeling_term mu i | i <- bnodes_ts ts1] by rewrite (perm_uniq e) //.
+                  have urtbs : uniq (get_bs [seq relabeling_term [eta mu] i | i <- bnodes_ts ts1]).
+                  by rewrite -undup_get_bsC // undup_uniq.
+                  have mem_eq_rt : get_bs [seq relabeling_term [eta mu] i | i <- bnodes_ts ts1] =i get_bs (bnodes_ts ts2).
+                  by move=> x; rewrite -!bnode_memP; apply perm_mem.
+                  by rewrite uniq_perm //.
+               + apply /eqP; rewrite eq_sym; apply /eqP.
+                 suffices contra:  perm_eq (get_bs [seq relabeling_term mu i | i <- bnodes_ts ts1]) (get_bs (bnodes_ts ts2)) -> perm_eq [seq relabeling_term mu i | i <- bnodes_ts ts1] (bnodes_ts ts2).
+                 by apply (contra_notF contra); rewrite e.
+
+                 move=> contr; apply uniq_perm=> //.
+                 by rewrite -(all_bnodes_uniq_bs (map_rel_bnode mu (all_bnodes_ts ts1))) // (perm_uniq contr).
+                 have alb := map_rel_bnode mu (all_bnodes_ts ts1).
+                 move=> [] //= b ; rewrite ?i_in_bnodes_ts ?l_in_bnodes_ts.
+                 have F: Iri b \in [seq relabeling_term mu i | i <- bnodes_ts ts1] -> negb (all (is_bnode (L:=L)) [seq relabeling_term mu i | i <- bnodes_ts ts1]).
+                 by move=> contra2; apply /allPn; exists (Iri b).
+                 by apply (contra_notF F); rewrite alb.
+                 have F: Lit b \in [seq relabeling_term mu i | i <- bnodes_ts ts1] -> negb (all (is_bnode (L:=L)) [seq relabeling_term mu i | i <- bnodes_ts ts1]).
+                 by move=> contra2; apply /allPn; exists (Lit b).
+                 apply (contra_notF F); rewrite alb //.
+                 by rewrite !bnode_memP (perm_mem contr).
+        Qed.
+
+        Lemma perm_relabel_bts ts1 ts2 mu :
+          perm_eq (map (relabeling_term mu) (bnodes_ts ts1)) (bnodes_ts ts2) =
+            perm_eq (map mu (get_bts ts1)) (get_bts ts2).
+        Proof. by rewrite perm_relabel_bnodes_ts. Qed.
+
+        Lemma perm_eq_bnodes_relabel ts1 ts2 mu :
+          perm_eq (get_bs (bnodes_ts (relabeling_seq_triple mu ts1))) (get_bs (bnodes_ts ts2)) ->
+          perm_eq (undup [seq mu i | i <- get_bs (bnodes_ts ts1)]) (get_bs (bnodes_ts ts2)).
+        Proof. move=> /perm_mem peqb; apply (uniq_perm (undup_uniq _))=> // x; rewrite -peqb{peqb ts2} mem_undup.
+               elim: ts1=> [//| h t IHts].
+               rewrite !bnodes_ts_cons -!undup_get_bs mem_undup -mem_map_undup -!get_bs_cat map_cat !mem_cat /= IHts; f_equal.
+               case: h=> [[]]// a []// b []// c ? ?; rewrite /bnodes_triple/terms_triple ?filter_undup //.
+               have ->:  [seq x <- [:: relabeling_term mu (Bnode a); relabeling_term mu (Iri b);
+                              relabeling_term mu (Bnode c)]
+                         | is_bnode x] = [:: (Bnode (mu a)); (Bnode (mu c))].
+               by [].
+               by rewrite -!undup_get_bs -mem_map_undup mem_undup.
+        Qed.
+
+        Lemma perm_eq_bts_relabel ts1 ts2 mu :
+          perm_eq (get_bts (relabeling_seq_triple mu ts1)) (get_bts ts2) ->
+          perm_eq (undup [seq mu i | i <- get_bts ts1]) (get_bts ts2).
+        Proof. by apply perm_eq_bnodes_relabel. Qed.
+
+        Lemma perm_eq_bnodes_relabel_inj_in ts1 ts2 mu :
+          {in (get_bs (bnodes_ts ts1))&, injective mu} ->
+          perm_eq (get_bs (bnodes_ts (relabeling_seq_triple mu ts1))) (get_bs (bnodes_ts ts2)) ->
+          perm_eq [seq mu i | i <- get_bs (bnodes_ts ts1)] (get_bs (bnodes_ts ts2)).
+        Proof. by move=> inj /perm_eq_bnodes_relabel/perm_undup_map_inj ->. Qed.
+
+        Lemma perm_eq_bts_relabel_inj_in ts1 ts2 mu :
+          {in (get_bts ts1)&, injective mu} ->
+          perm_eq (get_bts (relabeling_seq_triple mu ts1)) (get_bts ts2) ->
+          perm_eq [seq mu i | i <- get_bts ts1] (get_bts ts2).
+        Proof. by apply perm_eq_bnodes_relabel_inj_in. Qed.
+
+        Lemma relabeling_term_inj_terms_ts {B2 : eqType} (mu : B -> B2) ts sx sy :
+          {in get_bts ts &, injective mu} ->
+          sx \in terms_ts ts -> sy \in terms_ts ts ->
+                                  relabeling_term mu sx = relabeling_term mu sy ->
+                                  sx = sy.
+        Proof. case sx; case sy=> /= // bx b_y mu_inj memx memy.
+               by move=> [->].
+               by move=> [->].
+               by move=> [/mu_inj]-> //; rewrite -!bnode_memP !bterms_ts.
+        Qed.
+
+        Lemma inj_get_bts_inj_ts {B2: eqType} ts (mu : B -> B2) : ({in get_bts ts &, injective mu}) -> {in ts &, injective (relabeling_triple mu)}.
+        Proof.
+          move=> mu_inj; case=> sx ps ox ? ?; case=> sy py oy ? ? /= /mem_triple_terms_ts /= /and3P[memsx mempx memox] /mem_triple_terms_ts /= /and3P[memsy mempy memoy] [] eqs eqp eqo.
+            by apply triple_inj=> /=; apply (relabeling_term_inj_terms_ts mu_inj)=> //.
+        Qed.
+
+        Lemma can_bts_can_rtbs ts (mu nu: B -> B) : {in get_bts ts, nu \o mu =1 id} ->
+                                               {in ts, [eta relabeling_triple (nu \o mu)] =1 id}.
+        Proof. by apply can_bs_can_rtbs. Qed.
+
+
+      End Bnodes_ts.
+
+      Section Rdf_terms.
+
+        Definition terms {i b l : eqType} (g : rdf_graph i b l) : seq (term i b l) :=
+          undup (flatten (map (@terms_triple i b l) (graph g))).
+
+        Lemma terms_graph {i b l: eqType} (g : rdf_graph i b l) :
+          terms g = terms_ts (graph g).
+        Proof. by case g. Qed.
+
+        Lemma undup_terms g : undup (terms g) = (terms g).
+        Proof. by rewrite terms_graph undup_terms_ts. Qed.
+
+        Lemma uniq_terms {i b l : eqType} (g : rdf_graph i b l) : uniq (terms g).
+        Proof. by apply undup_uniq. Qed.
+        Hint Resolve uniq_terms.
+
+        Lemma terms_cons {i b l : eqType} (trpl : triple i b l) (ts : seq (triple i b l)) (us : uniq (trpl :: ts)):
+          terms (mkRdfGraph us) = undup (terms_triple trpl ++ (terms (mkRdfGraph (uniq_tail us)))).
+        Proof. by rewrite !terms_graph terms_ts_cons. Qed.
+
+        Lemma mem_triple_terms t g: t \in g -> [&& (subject t) \in (terms g),
+              ((predicate t) \in (terms g)) & ((object t) \in terms g)].
+      Proof. by rewrite terms_graph; apply mem_triple_terms_ts. Qed.
+
+
+      End Rdf_terms.
 
     Section TermRelabeling.
       Variable B1 B2: eqType.
-
-      Lemma terms_triple_map_rt (t : triple I B1 L) (mu : B1 -> B2) :
-        terms_triple (relabeling_triple mu t) =i [seq relabeling_term mu i | i <- terms_triple t].
-      Proof. by case t=> s p o ? ? x; rewrite -mem_map_undup mem_undup. Qed.
-
-      Lemma terms_ts_relabeled_mem (ts : seq (triple I B1 L)) (mu: B1 -> B2) :
-        (terms_ts (relabeling_seq_triple mu ts)) =i (map (relabeling_term mu) (terms_ts ts)).
-      Proof. elim: ts=> [//| h t IHt] /= x.
-             by rewrite !terms_ts_cons !mem_undup -mem_map_undup map_cat !mem_cat IHt terms_triple_map_rt.
-      Qed.
 
       Lemma terms_relabeled_mem (g : rdf_graph I B1 L) (mu: B1 -> B2) :
         forall us,
         (@terms I B2 L (@relabeling B1 B2 mu g us)) =i (map (relabeling_term mu) (terms g)).
       Proof. by move=> ? x; rewrite !terms_graph terms_ts_relabeled_mem. Qed.
-
-      Lemma relabeling_triple_inj (i l b1 b2 : Type) (mu : b1 -> b2) (mu_inj :injective mu) : injective (@relabeling_triple i l b1 b2 mu).
-      Proof.
-        have /(_ i l) rtmu_inj := (relabeling_term_inj mu_inj).
-        by move=> [? ? ? ? ?] [? ? ? ? ?] // [] /rtmu_inj eq1 /rtmu_inj eq2 /rtmu_inj eq3; apply triple_inj.
-      Qed.
-
-      Lemma terms_ts_relabeled (ts : seq (triple I B1 L)) (mu : B1 -> B2) (mu_inj: injective mu):
-        terms_ts (relabeling_seq_triple mu ts) = [seq relabeling_term mu i | i <- terms_ts ts].
-      Proof.
-        have rts_inj := (@relabeling_triple_inj I L B1 B2 mu mu_inj).
-        have rt_inj := (@relabeling_term_inj I B1 B2 L mu mu_inj).
-        elim: ts=> [//| h tl IHtl].
-        have step: undup ([seq relabeling_term mu i | i <- terms_triple h] ++
-                          [seq relabeling_term mu i | i <- flatten [seq terms_triple i | i <- tl]]) =
-               undup
-                 ([seq relabeling_term mu i | i <- terms_triple h] ++
-                    undup [seq relabeling_term mu i | i <- flatten [seq terms_triple i | i <- tl]]) by rewrite undup_cat_r.
-        rewrite -undup_map_inj // !terms_ts_cons /= map_cat step.
-        by apply f_equal; rewrite IHtl terms_relabeled_triple // undup_map_inj.
-      Qed.
 
       Lemma terms_relabeled (g : rdf_graph I B1 L) (mu: B1 -> B2) (inj_mu : injective mu):
         forall us,
@@ -230,101 +505,11 @@ Section Rdf.
 
     End TermRelabeling.
 
-    Definition bnodes_ts (i b l : eqType) (ts : seq (triple i b l)): seq (term i b l) :=
-      undup (filter (@is_bnode i b l) (terms_ts ts)).
-
     Definition bnodes (i b l : eqType) (g : rdf_graph i b l) : seq (term i b l) :=
       bnodes_ts (graph g).
 
-    Section BnodeRelabeling.
-      Variable B1 B2: eqType.
-
-      (* Lemma mem_filter_map ts1 ts2 : *)
-      (*   filter *)
-      Lemma rt_pres_b (t : term I B1 L) (mu : B1 -> B2) : is_bnode t -> is_bnode (relabeling_term mu t).
-      Proof. by case t. Qed.
-
-      Lemma mem_filter_map (T : eqType) f p a (s : seq T) :
-        (forall b, p b = p (f b)) -> (a \in (map f (filter p s))) = (a \in filter p (map f s)).
-      Proof. elim: s=> [//|h t IHts] pres.
-             by case e: (p h); rewrite /= e; rewrite pres in e; rewrite e /= ?in_cons IHts //.
-      Qed.
-
-      Lemma filter_map_rt (trms: seq (term I B1 L)) (us: uniq trms) (mu: B1 -> B2) :
-        [seq x <- [seq relabeling_term mu i | i <- trms ] | is_bnode x] =i
-                                                                         [seq relabeling_term mu i | i <- trms & is_bnode i].
-      Proof. elim: trms us=> [//| hd tl IHtl] [/andP[nin utl]] x /=.
-             case e: (is_bnode hd) nin.
-             by rewrite rt_pres_b //= in_cons IHtl.
-             have -> : is_bnode (relabeling_term mu hd) = false by move : e; case hd=> //.
-             by rewrite IHtl.
-      Qed.
-
-      Lemma bnodes_ts_relabel_mem (ts : seq (triple I B1 L)) (mu: B1 -> B2) :
-        bnodes_ts (relabeling_seq_triple mu ts) =i (map (relabeling_term mu) (bnodes_ts ts)).
-      Proof. move=> x; rewrite mem_undup -mem_map_undup.
-             by rewrite mem_filter terms_ts_relabeled_mem -mem_filter filter_map_rt.
-      Qed.
-
-      Lemma bnodes_relabel_mem (g: rdf_graph I B1 L) (mu: B1 -> B2) :
-        forall us,
-        bnodes (@relabeling B1 B2 mu g us) =i (map (relabeling_term mu) (bnodes g)).
-      Proof. by move=> ? x; rewrite bnodes_ts_relabel_mem. Qed.
-
-      Lemma bnodes_ts_relabel_inj (ts: seq (triple I B1 L)) (mu: B1 -> B2) (mu_inj : injective mu):
-        bnodes_ts (relabeling_seq_triple mu ts) = (map (relabeling_term mu) (bnodes_ts ts)).
-      Proof.
-        have /(_ I L) rtmu_inj := relabeling_term_inj mu_inj.
-        rewrite /bnodes_ts terms_ts_relabeled // -filter_undup undup_map_inj // -filter_undup.
-        elim: (undup (terms_ts ts)) => [// | hd tl IHtl] /=.
-             case e: (is_bnode hd).
-             by rewrite rt_pres_b // IHtl.
-             have -> : is_bnode (relabeling_term mu hd) = false by move : e; case hd=> //.
-             by rewrite IHtl.
-      Qed.
-
-      (* Lemma undup_map_inj_in (T1 T2 : eqType) (f : T1 -> T2) (s : seq T1) : *)
-      (*   {in s&, injective f} -> *)
-      (*   undup [seq f i | i <- s] =i [seq f i | i <- undup s]. *)
-      (* Proof. *)
-      (*   move=> inj_f. *)
-      (*   move=> x; rewrite -mem_map_undup mem_undup. *)
-
-      (*   elim: s => //= h t IHt injF. *)
-      (*   case e: (h \in t). *)
-      (*   by rewrite map_f // IHt // => x y /(inweak h) xin /(inweak h) yin; apply injF. *)
-      (*   case e2: (f h \in [seq f i | i <- t]). *)
-      (*   rewrite (map_f f).  in e. rewrite e. *)
-
-
-      (*   /=. *)
-      Lemma bnodes_relabel (g: rdf_graph I B1 L) (mu: B1 -> B2) (inj_mu : injective mu):
-        forall us,
-          bnodes (@relabeling B1 B2 mu g us) = (map (relabeling_term mu) (bnodes g)).
-      Proof. by rewrite /bnodes /= bnodes_ts_relabel_inj. Qed.
-
-    End BnodeRelabeling.
-
-    Lemma bnodes_ts_cons (trpl : triple I B L) (ts : seq (triple I B L)) :
-      bnodes_ts (trpl :: ts) = undup ((bnodes_triple trpl) ++ (bnodes_ts ts)).
-    Proof. by rewrite /bnodes_ts terms_ts_cons filter_undup undup_idem undup_cat_r filter_cat. Qed.
-
-    Lemma bnodes_cons (trpl : triple I B L) (ts : seq (triple I B L)) :
-      forall us : uniq (trpl :: ts),
-        bnodes {| graph := trpl :: ts; ugraph := us |} = undup ((bnodes_triple trpl) ++ (bnodes {| graph := ts; ugraph := uniq_tail us |})).
-    Proof. by rewrite /bnodes/= bnodes_ts_cons. Qed.
-
     Remark undup_bnodes g : undup (bnodes g) = bnodes g.
     Proof. exact: undup_idem. Qed.
-
-    Lemma all_bnodes_ts ts : all (@is_bnode I B L) (bnodes_ts ts).
-    Proof. elim: ts=> [// | t ts IHts].
-           by rewrite bnodes_ts_cons all_undup all_cat IHts Bool.andb_true_r all_bnodes_triple_is_bnode.
-    Qed.
-
-    Lemma all_bnodes_perm ts s:
-      perm_eq (bnodes_ts ts) s -> forall x, x \in s -> is_bnode x.
-    Proof. by move=> peq x xin; apply (in_all xin); rewrite -(perm_all _ peq) all_bnodes_ts. Qed.
 
     Lemma all_bnodes g : all (@is_bnode I B L) (bnodes g).
     Proof. by rewrite all_bnodes_ts. Qed.
@@ -338,19 +523,14 @@ Section Rdf.
       by apply in_bnodes.
     Qed.
 
-    Lemma uniq_bnodes_ts ts : uniq (bnodes_ts ts).
-    Proof. exact: undup_uniq. Qed.
-    Hint Resolve uniq_bnodes_ts.
+    Lemma bnodes_cons (trpl : triple I B L) (ts : seq (triple I B L)) :
+      forall us : uniq (trpl :: ts),
+        bnodes {| graph := trpl :: ts; ugraph := us |} = undup ((bnodes_triple trpl) ++ (bnodes {| graph := ts; ugraph := uniq_tail us |})).
+    Proof. by rewrite /bnodes/= bnodes_ts_cons. Qed.
 
     Lemma uniq_bnodes g : uniq (bnodes g).
     Proof. exact: undup_uniq. Qed.
     Hint Resolve uniq_bnodes.
-
-    Lemma i_in_bnodes_ts id ts: Iri id \in bnodes_ts ts = false.
-    Proof. by rewrite /bnodes_ts -filter_undup mem_filter. Qed.
-
-    Lemma l_in_bnodes_ts l ts: Lit l \in bnodes_ts ts = false.
-    Proof. by rewrite /bnodes_ts -filter_undup mem_filter. Qed.
 
     Lemma i_in_bnodes id g: Iri id \in bnodes g = false.
     Proof. by rewrite /bnodes i_in_bnodes_ts. Qed.
@@ -358,69 +538,82 @@ Section Rdf.
     Lemma l_in_bnodes l g: Lit l \in bnodes g = false.
     Proof. by rewrite /bnodes l_in_bnodes_ts. Qed.
 
-    Definition get_bts {i b l : eqType} (ts : seq (triple i b l)) : seq b :=
-      get_bs (bnodes_ts ts).
+    Section BnodeRelabeling.
+      Variable B1 B2: eqType.
+
+      Lemma bnodes_relabel_mem (g: rdf_graph I B1 L) (mu: B1 -> B2) :
+        forall us,
+        bnodes (@relabeling B1 B2 mu g us) =i (map (relabeling_term mu) (bnodes g)).
+      Proof. by move=> ? x; rewrite bnodes_ts_relabel_mem. Qed.
+
+      Lemma bnodes_relabel (g: rdf_graph I B1 L) (mu: B1 -> B2) (inj_mu : injective mu):
+        forall us,
+          bnodes (@relabeling B1 B2 mu g us) = (map (relabeling_term mu) (bnodes g)).
+      Proof. by rewrite /bnodes /= bnodes_ts_relabel_inj. Qed.
+
+      Lemma bterms b g: Bnode b \in (terms g) -> Bnode b \in (bnodes g).
+      Proof. by rewrite terms_graph; apply bterms_ts. Qed.
+
+    End BnodeRelabeling.
+    End Terms_ts.
 
     Definition get_b g : seq B :=
       get_bts g.
 
-    Lemma bnode_memP (i b1 l: eqType) (b : b1) trms : Bnode b \in trms = (b \in @get_bs i b1 l trms).
-    Proof. elim: trms=> [//| h t' IHt].
-           by case: h=> // ?; rewrite !in_cons IHt eqb_eq.
-    Qed.
 
-    Lemma bnode_memPn (i b1 l: eqType) (b : b1) trms : Bnode b \notin trms = (b \notin @get_bs i b1 l trms).
-    Proof. by rewrite /negb bnode_memP. Qed.
-
-    Lemma get_bs_of_uniq (s : seq (term I B L)) : uniq s -> get_bs (undup s) = get_bs s.
-    Proof. rewrite /get_bs. elim: s=> [//| h t IHl]; rewrite cons_uniq=> /andP[/eqP nin unt] /=.
-           by case: (h \in t) nin => //; case: h=> x /= _; rewrite IHl.
-    Qed.
-
-    Lemma undup_get_bsC (s : seq (term I B L)) : uniq s -> (undup (get_bs s)) = get_bs s.
-    Proof. elim: s=> [//| h t IHt].
-           move=> /andP[nin unt] /=; case: h nin=> //= b; rewrite ?IHt //.
-           by rewrite bnode_memPn /negb; case: (b \in get_bs t)=> //; by rewrite IHt.
-    Qed.
-
-    Lemma uniq_get_bs ts : uniq (get_bs (bnodes_ts ts)).
-    Proof. by rewrite -(undup_get_bsC (uniq_bnodes_ts ts)) undup_uniq. Qed.
-    Hint Resolve uniq_get_bs.
-
-    Lemma uniq_get_bts ts : uniq (get_bts ts).
-    Proof. by rewrite /get_b uniq_get_bs. Qed.
-    Hint Resolve uniq_get_bts.
+    Lemma relabeling_term_inj_terms {B2 : eqType} (mu : B -> B2) g sx sy :
+      {in get_b g &, injective mu} ->
+      sx \in terms g -> sy \in terms g ->
+                              relabeling_term mu sx = relabeling_term mu sy ->
+                              sx = sy.
+    Proof. apply relabeling_term_inj_terms_ts. Qed.
 
     Lemma uniq_get_b g : uniq (get_b g).
     Proof. by rewrite /get_b uniq_get_bs. Qed.
     Hint Resolve uniq_get_b.
 
-    Lemma relabeling_triple_of_comp (B1 B2 B3: eqType)(mu : B2 -> B3) (nu : B1 -> B2):
-      ((@relabeling_triple I L _ _ mu) \o (@relabeling_triple I L _ _ nu)) =1 (relabeling_triple (mu \o nu)).
-    Proof. by move=> t; rewrite relabeling_triple_comp. Qed.
+    Lemma bnodes_map_get_b g : bnodes g = map (fun b=> Bnode b) (get_b g).
+    Proof. by rewrite /bnodes -bnodes_map_get_bs. Qed.
 
-    Lemma bijective_perm_eq_relabeling_st mu nu ts1 ts2 :
-      uniq (relabeling_seq_triple nu ts1) ->
-      cancel mu nu -> perm_eq (relabeling_seq_triple mu ts2) ts1 -> perm_eq ts2 (relabeling_seq_triple nu ts1).
-      Proof. move=> urtnu can_munu /(perm_map (relabeling_triple nu)) peq.
-             have can_id: {in ts2, [eta relabeling_triple (nu \o mu)] =1 id}.
-             by move=>  [[]s []p []o ? ?] _ //; apply triple_inj=> //=; rewrite can_munu.
-             have peq_can: perm_eq ts2 [seq relabeling_triple nu i | i <- relabeling_seq_triple mu ts2].
-             by rewrite relabeling_triple_map_comp map_id_in //.
-             apply: perm_trans peq_can peq.
-      Qed.
+    Lemma perm_relabel_bnodes g1 g2 mu :
+      perm_eq (map (relabeling_term mu) (bnodes g1)) (bnodes g2) =
+        perm_eq (map mu (get_b g1)) (get_b g2).
+    Proof. by rewrite perm_relabel_bnodes_ts. Qed.
 
-    Lemma bijective_eqb_rdf mu nu g1 g2 :
-      forall us1 us2,
-        cancel mu nu -> eqb_rdf (@relabeling _ _ mu g2 us1) g1 -> eqb_rdf g2 (@relabeling _ _ nu g1 us2).
+    Lemma inj_get_b_inj_g {B2: eqType} g (mu : B -> B2) : ({in get_b g &, injective mu}) -> {in g &, injective (relabeling_triple mu)}.
     Proof.
-      by move=> us1 us2 can_munu; rewrite /eqb_rdf/relabeling/=; apply bijective_perm_eq_relabeling_st.
+      move=> mu_inj; case=> sx ps ox ? ?; case=> sy py oy ? ? /= /mem_triple_terms /= /and3P[memsx mempx memox] /mem_triple_terms /= /and3P[memsy mempy memoy] [] eqs eqp eqo.
+        by apply triple_inj=> /=; apply (relabeling_term_inj_terms mu_inj)=> //.
     Qed.
+
+
+    Lemma map_comp_in_id g (mu nu: B -> B) : [seq (nu \o mu) i | i <- get_b g] = get_b g ->
+                                            {in (get_b g), nu \o mu =1 id}.
+    Proof. elim: (get_b g)=> [| h t IHtl]; first by move=> _ x; rewrite in_nil //.
+           move=> [heq teq] x; rewrite in_cons; case e: (x == h)=> /=.
+           + by move: e=> /eqP ->; rewrite heq.
+           + apply IHtl; apply teq.
+    Qed.
+
+    Lemma bterm_eq_mem_get_b (b: B) g :
+      (@Bnode I B L b) \in terms g ->
+                           b \in get_b g.
+    Proof. by rewrite terms_graph/get_b; apply bterm_eq_mem_get_bs. Qed.
+
+    Lemma mem_g_mem_triple_b t g b : t \in g -> Bnode b \in bnodes_triple t -> b \in get_b g.
+    Proof. by apply mem_ts_mem_triple_bs. Qed.
+
+    Lemma can_b_can_rtb g (mu nu: B -> B) : {in get_b g, nu \o mu =1 id} ->
+                          {in g, [eta relabeling_triple (nu \o mu)] =1 id}.
+    Proof. by apply can_bs_can_rtbs. Qed.
 
     Remark id_bij T: bijective (@id T). Proof. by exists id. Qed.
     Hint Resolve id_bij.
 
     Section Isomorphism.
+      Hint Resolve uniq_get_bts.
+      Hint Resolve uniq_bnodes_ts.
+      Hint Resolve uniq_get_bs.
 
       Section PreIsomorphism.
 
@@ -506,6 +699,39 @@ Section Rdf.
         Lemma pre_iso_trans g1 g2 g3 : pre_iso g1 g2 -> pre_iso g2 g3 -> pre_iso g1 g3.
         Proof. by apply pre_iso_ts_trans. Qed.
 
+        Lemma is_pre_iso_ts_inj ts1 ts2 mu : is_pre_iso_ts ts1 ts2 mu -> {in get_bts ts1 &, injective mu}.
+        Proof.
+        move=> hmu b b' hb1 hb'.
+        apply: contra_eq => neqb.
+        apply/negP=> eqmu.
+        have test : perm_eq (get_bts ts1)  (b' :: rem b' (get_bts ts1)).
+          by apply: perm_to_rem.
+        have {test} /(perm_map mu) /= test : perm_eq (get_bts ts1)  (b' :: b :: rem b (rem b' (get_bts ts1))).
+          apply: perm_trans test _. rewrite perm_cons. apply: perm_to_rem.
+          by rewrite mem_rem_uniq // inE neqb.
+        have hcount : 2 <= count_mem (mu b) (map mu (get_bts ts1)).
+          by move/permP: test->; rewrite /= (eqP eqmu) !eqxx.
+        have {hcount} : 2 <= count_mem (mu b) (get_bts ts2).
+          by move/permP: hmu<-.
+        by rewrite count_uniq_mem //; case: (mu b \in get_bts ts2).
+        Qed.
+
+        Lemma is_pre_iso_inj g1 g2 mu : is_pre_iso g1 g2 mu -> {in get_b g1 &, injective mu}.
+        Proof. by apply is_pre_iso_ts_inj. Qed.
+
+        Lemma is_pre_iso_ts_bnodes_inj ts1 ts2 mu : is_pre_iso_ts ts1 ts2 mu -> {in bnodes_ts ts1 &, injective (relabeling_term mu)}.
+        Proof. move=> /is_pre_iso_ts_inj hmu []b // []b' //=;
+               rewrite bnodes_map_get_bs !mem_map // => hb1 hb' []=> eq; rewrite ?eq //.
+               by congr Bnode; apply hmu.
+        Qed.
+
+        Lemma is_pre_iso_bnodes_inj g1 g2 mu : is_pre_iso g1 g2 mu -> {in bnodes g1 &, injective (relabeling_term mu)}.
+        Proof. by apply is_pre_iso_ts_bnodes_inj. Qed.
+
+        Lemma uniq_relabeling_pre_iso mu (ts : seq (triple I B L)):
+          uniq ts -> is_pre_iso_ts ts (relabeling_seq_triple mu ts) mu -> uniq (relabeling_seq_triple mu ts).
+        Proof. by rewrite /is_pre_iso_ts=> uts /is_pre_iso_ts_inj/inj_get_bts_inj_ts ?; rewrite map_inj_in_uniq //. Qed.
+
       End PreIsomorphism.
 
       Definition is_iso_ts ts1 ts2 mu :=
@@ -522,7 +748,7 @@ Section Rdf.
       Definition iso g1 g2 := iso_ts g1 g2.
       (* exists mu, @is_iso g1 g2 mu. *)
 
-      Remark is_iso_is_pre_iso g1 g2 mu: @is_iso g1 g2 mu -> is_pre_iso g1 g2 mu.
+      Remark is_iso_is_pre_iso g1 g2 mu: is_iso g1 g2 mu -> is_pre_iso g1 g2 mu.
       Proof. by case/and3P. Qed.
 
       Definition iso_refl g : iso g g.
@@ -531,90 +757,28 @@ Section Rdf.
              by rewrite /is_iso_ts relabeling_seq_triple_id ug  /= /is_pre_iso/is_pre_iso_ts map_id !perm_refl.
       Qed.
 
-      Lemma eqb_rdf_terms g1 g2 : eqb_rdf g1 g2 -> perm_eq (terms g1) (terms g2).
-      Proof. rewrite /eqb_rdf/terms=> peq.
-             by rewrite perm_undup //; apply perm_mem; rewrite perm_flatten //; apply: perm_map peq.
-      Qed.
+      Section eqb_rdf_perm_eq.
+        (* TODO find a place for these lemmas *)
+        Lemma eqb_rdf_terms g1 g2 : eqb_rdf g1 g2 -> perm_eq (terms g1) (terms g2).
+        Proof. rewrite /eqb_rdf/terms=> peq.
+               by rewrite perm_undup //; apply perm_mem; rewrite perm_flatten //; apply: perm_map peq.
+        Qed.
 
-      Lemma eqb_rdf_bnodes g1 g2 : eqb_rdf g1 g2 -> perm_eq (bnodes g1) (bnodes g2).
-      Proof. move=> /eqb_rdf_terms eqb.
-             by rewrite /bnodes perm_undup //; apply: perm_mem; apply: perm_filter.
-      Qed.
+        Lemma eqb_rdf_bnodes g1 g2 : eqb_rdf g1 g2 -> perm_eq (bnodes g1) (bnodes g2).
+        Proof. move=> /eqb_rdf_terms eqb.
+               by rewrite /bnodes perm_undup //; apply: perm_mem; apply: perm_filter.
+        Qed.
 
-      Lemma eqb_rdf_get_b g1 g2 : eqb_rdf g1 g2 -> perm_eq (get_b g1) (get_b g2).
-      Proof. by move=> /eqb_rdf_bnodes eqb ; rewrite /get_b/get_bs; apply: perm_pmap eqb. Qed.
+        Lemma eqb_rdf_get_b g1 g2 : eqb_rdf g1 g2 -> perm_eq (get_b g1) (get_b g2).
+        Proof. by move=> /eqb_rdf_bnodes eqb ; rewrite /get_b/get_bs; apply: perm_pmap eqb. Qed.
 
-      Lemma terms_uniq g : uniq (terms g).
-      Proof. by apply undup_uniq. Qed.
+        Lemma eqb_rdf_get_b_hom g1 g2 mu us :
+          eqb_rdf (@relabeling _ _ mu g1 us) g2 -> perm_eq (undup (map mu (get_b g1))) (get_b g2).
+        Proof.
+          by move=> /eqb_rdf_get_b eqb ; rewrite /get_b/bnodes/relabeling (perm_eq_bnodes_relabel eqb).
+        Qed.
 
-      Lemma bnodes_map_get_bs ts : bnodes_ts ts = map (fun b=> Bnode b) (get_bs (bnodes_ts ts)).
-      Proof.
-        move: (all_bnodes_ts ts).
-        rewrite /get_b/bnodes/bnodes_ts filter_undup // undup_idem -filter_undup.
-        elim: [seq x <- undup (flatten [seq terms_triple i | i <- ts]) | is_bnode x]=> [//| []//=b t IHt] al.
-        by rewrite -IHt.
-      Qed.
-
-      Lemma bnodes_map_get_bts ts : bnodes_ts ts = map (fun b=> Bnode b) (get_bts ts).
-      Proof. exact: bnodes_map_get_bs. Qed.
-
-      Lemma bnodes_map_get_b g : bnodes g = map (fun b=> Bnode b) (get_b g).
-      Proof. by rewrite /bnodes -bnodes_map_get_bs. Qed.
-
-      Lemma count_mem_bnodes b l: all (@is_bnode I B L) l -> count_mem b (get_bs l) = count_mem (Bnode b) l.
-      Proof. elim: l=> [//|[]//b' t IHt] albn.
-             by rewrite /= eqb_eq /eqb_term /= IHt.
-      Qed.
-
-      Lemma perm_eq_1s (b1 b2: B) : perm_eq [:: b1] [:: b2] = perm_eq [:: (@Bnode I B L b1)] [:: Bnode b2].
-      Proof. by rewrite /perm_eq /= !eqb_eq /=. Qed.
-
-      Lemma get_bs_map s mu: all (@is_bnode I B L) s -> (@get_bs I B L (map (relabeling_term mu) s)) = map mu (get_bs s).
-      Proof. by elim: s=> [//| []//b t IHtl] /==> ? ; rewrite IHtl. Qed.
-
-      Lemma map_rel_bnode s mu: all (@is_bnode I B L) s -> all (@is_bnode I B L) (map (relabeling_term mu) s).
-      Proof. by elim: s=> [//| []//b t IHt]. Qed.
-
-      Lemma all_bnodes_uniq_bs (i b l : eqType) s: all (@is_bnode i b l) s -> uniq (get_bs s) = uniq s.
-      Proof. by elim: s=> [//| []//ab t IHt] alb; rewrite /= IHt // bnode_memPn. Qed.
-
-      Lemma perm_relabel_bnodes_ts ts1 ts2 mu :
-      perm_eq [seq relabeling_term mu i | i <- bnodes_ts ts1] (bnodes_ts ts2) =
-        perm_eq [seq mu i | i <- get_bs (bnodes_ts ts1)] (get_bs (bnodes_ts ts2)).
-      Proof. rewrite -(get_bs_map mu (all_bnodes_ts ts1)).
-             case e : (perm_eq [seq relabeling_term mu i | i <- bnodes_ts ts1] (bnodes_ts ts2)).
-             +  have urt_l : uniq [seq relabeling_term mu i | i <- bnodes_ts ts1] by rewrite (perm_uniq e) //.
-                have urtbs : uniq (get_bs [seq relabeling_term [eta mu] i | i <- bnodes_ts ts1]).
-                by rewrite -undup_get_bsC // undup_uniq.
-                have mem_eq_rt : get_bs [seq relabeling_term [eta mu] i | i <- bnodes_ts ts1] =i get_bs (bnodes_ts ts2).
-                by move=> x; rewrite -!bnode_memP; apply perm_mem.
-                by rewrite uniq_perm //.
-             + apply /eqP; rewrite eq_sym; apply /eqP.
-               suffices contra:  perm_eq (get_bs [seq relabeling_term mu i | i <- bnodes_ts ts1]) (get_bs (bnodes_ts ts2)) -> perm_eq [seq relabeling_term mu i | i <- bnodes_ts ts1] (bnodes_ts ts2).
-               by apply (contra_notF contra); rewrite e.
-
-               move=> contr; apply uniq_perm=> //.
-               by rewrite -(all_bnodes_uniq_bs (map_rel_bnode mu (all_bnodes_ts ts1))) // (perm_uniq contr).
-               have alb := map_rel_bnode mu (all_bnodes_ts ts1).
-               move=> [] //= b ; rewrite ?i_in_bnodes_ts ?l_in_bnodes_ts.
-               have F: Iri b \in [seq relabeling_term mu i | i <- bnodes_ts ts1] -> negb (all (is_bnode (L:=L)) [seq relabeling_term mu i | i <- bnodes_ts ts1]).
-               by move=> contra2; apply /allPn; exists (Iri b).
-               by apply (contra_notF F); rewrite alb.
-               have F: Lit b \in [seq relabeling_term mu i | i <- bnodes_ts ts1] -> negb (all (is_bnode (L:=L)) [seq relabeling_term mu i | i <- bnodes_ts ts1]).
-               by move=> contra2; apply /allPn; exists (Lit b).
-               apply (contra_notF F); rewrite alb //.
-               by rewrite !bnode_memP (perm_mem contr).
-      Qed.
-
-      Lemma perm_relabel_bts ts1 ts2 mu :
-        perm_eq (map (relabeling_term mu) (bnodes_ts ts1)) (bnodes_ts ts2) =
-          perm_eq (map mu (get_bts ts1)) (get_bts ts2).
-      Proof. by rewrite perm_relabel_bnodes_ts. Qed.
-
-      Lemma perm_relabel_bnodes g1 g2 mu :
-        perm_eq (map (relabeling_term mu) (bnodes g1)) (bnodes g2) =
-          perm_eq (map mu (get_b g1)) (get_b g2).
-      Proof. by rewrite perm_relabel_bnodes_ts. Qed.
+      End eqb_rdf_perm_eq.
 
       Remark eqiso g1 g2 : eqb_rdf g1 g2 -> iso g1 g2.
       Proof.
@@ -623,218 +787,6 @@ Section Rdf.
         rewrite /is_iso/is_iso_ts usid /is_pre_iso/is_pre_iso_ts map_id relabeling_seq_triple_id /=; apply/andP; split=> //.
         - exact: eqb_rdf_get_b.
       Qed.
-
-      Lemma map_of_triples t1 ft (f : B -> B): relabeling_term f (subject t1) = (subject ft) ->
-                                                relabeling_term f (predicate t1) = predicate ft ->
-                                                relabeling_term f (object t1) = object ft
-                                                -> relabeling_triple f t1 = ft.
-      Proof. by move=> rts rtp rto; apply triple_inj; rewrite -?rts -?rtp -?rto; case t1. Qed.
-
-      Lemma is_pre_iso_ts_inj ts1 ts2 mu : is_pre_iso_ts ts1 ts2 mu -> {in get_bts ts1 &, injective mu}.
-      Proof.
-      move=> hmu b b' hb1 hb'.
-      apply: contra_eq => neqb.
-      apply/negP=> eqmu.
-      have test : perm_eq (get_bts ts1)  (b' :: rem b' (get_bts ts1)).
-        by apply: perm_to_rem.
-      have {test} /(perm_map mu) /= test : perm_eq (get_bts ts1)  (b' :: b :: rem b (rem b' (get_bts ts1))).
-        apply: perm_trans test _. rewrite perm_cons. apply: perm_to_rem.
-        by rewrite mem_rem_uniq // inE neqb.
-      have hcount : 2 <= count_mem (mu b) (map mu (get_bts ts1)).
-        by move/permP: test->; rewrite /= (eqP eqmu) !eqxx.
-      have {hcount} : 2 <= count_mem (mu b) (get_bts ts2).
-        by move/permP: hmu<-.
-      by rewrite count_uniq_mem //; case: (mu b \in get_bts ts2).
-      Qed.
-
-      Lemma is_pre_iso_inj g1 g2 mu : is_pre_iso g1 g2 mu -> {in get_b g1 &, injective mu}.
-      Proof. by apply is_pre_iso_ts_inj. Qed.
-
-      Lemma bnode_inj (i b l : eqType) : injective (fun bn=> @Bnode i b l bn).
-      Proof. by move=> x y; case. Qed.
-      Hint Resolve bnode_inj.
-
-      Lemma is_pre_iso_ts_bnodes_inj ts1 ts2 mu : is_pre_iso_ts ts1 ts2 mu -> {in bnodes_ts ts1 &, injective (relabeling_term mu)}.
-      Proof. move=> /is_pre_iso_ts_inj hmu []b // []b' //=;
-             rewrite bnodes_map_get_bs !mem_map // => hb1 hb' []=> eq; rewrite ?eq //.
-             by congr Bnode; apply hmu.
-      Qed.
-
-      Lemma is_pre_iso_bnodes_inj g1 g2 mu : is_pre_iso g1 g2 mu -> {in bnodes g1 &, injective (relabeling_term mu)}.
-      Proof. by apply is_pre_iso_ts_bnodes_inj. Qed.
-
-      Lemma undup_get_bs (s : seq (term I B L)) : (undup (get_bs s)) = (get_bs (undup s)).
-      Proof. elim: s=> [//|h t IHts] /=.
-             case e: (h \in t); first by move: e; case h=> //b; rewrite /= -IHts bnode_memP=> ->.
-             by move: e; case h=> //b; rewrite /= -IHts bnode_memP=> ->.
-      Qed.
-
-      Lemma get_bs_cat (s1 s2: seq (term I B L)): get_bs s1 ++ get_bs s2 = get_bs (s1 ++ s2).
-      Proof. by elim: s1 s2=> [//| []//=b t IHts] s2; rewrite IHts. Qed.
-
-      Lemma perm_eq_bnodes_relabel ts1 ts2 mu :
-        perm_eq (get_bs (bnodes_ts (relabeling_seq_triple mu ts1))) (get_bs (bnodes_ts ts2)) ->
-        perm_eq (undup [seq mu i | i <- get_bs (bnodes_ts ts1)]) (get_bs (bnodes_ts ts2)).
-      Proof. move=> /perm_mem peqb; apply (uniq_perm (undup_uniq _))=> // x; rewrite -peqb{peqb ts2} mem_undup.
-             elim: ts1=> [//| h t IHts].
-             rewrite !bnodes_ts_cons -!undup_get_bs mem_undup -mem_map_undup -!get_bs_cat map_cat !mem_cat /= IHts; f_equal.
-             case: h=> [[]]// a []// b []// c ? ?; rewrite /bnodes_triple/terms_triple ?filter_undup //.
-             have ->:  [seq x <- [:: relabeling_term mu (Bnode a); relabeling_term mu (Iri b);
-                            relabeling_term mu (Bnode c)]
-                       | is_bnode x] = [:: (Bnode (mu a)); (Bnode (mu c))].
-             by [].
-             by rewrite -!undup_get_bs -mem_map_undup mem_undup.
-      Qed.
-
-      Lemma perm_eq_bts_relabel ts1 ts2 mu :
-        perm_eq (get_bts (relabeling_seq_triple mu ts1)) (get_bts ts2) ->
-        perm_eq (undup [seq mu i | i <- get_bts ts1]) (get_bts ts2).
-      Proof. by apply perm_eq_bnodes_relabel. Qed.
-
-      Lemma perm_eq_bnodes_relabel_inj_in ts1 ts2 mu :
-        {in (get_bs (bnodes_ts ts1))&, injective mu} ->
-        perm_eq (get_bs (bnodes_ts (relabeling_seq_triple mu ts1))) (get_bs (bnodes_ts ts2)) ->
-        perm_eq [seq mu i | i <- get_bs (bnodes_ts ts1)] (get_bs (bnodes_ts ts2)).
-      Proof. by move=> inj /perm_eq_bnodes_relabel/perm_undup_map_inj ->. Qed.
-
-      Lemma perm_eq_bts_relabel_inj_in ts1 ts2 mu :
-        {in (get_bts ts1)&, injective mu} ->
-        perm_eq (get_bts (relabeling_seq_triple mu ts1)) (get_bts ts2) ->
-        perm_eq [seq mu i | i <- get_bts ts1] (get_bts ts2).
-      Proof. by apply perm_eq_bnodes_relabel_inj_in. Qed.
-
-      Lemma eqb_rdf_get_b_hom g1 g2 mu us :
-        eqb_rdf (@relabeling _ _ mu g1 us) g2 -> perm_eq (undup (map mu (get_b g1))) (get_b g2).
-      Proof.
-        by move=> /eqb_rdf_get_b eqb ; rewrite /get_b/bnodes/relabeling (perm_eq_bnodes_relabel eqb).
-      Qed.
-
-      Lemma mem_get_bs_undup (s: seq (term I B L)) : get_bs (undup s) =i get_bs s.
-      Proof. elim: s=> [//| h t IHts] x /=.
-             case e: (h \in t).
-             case: h e=> //= b.
-             by rewrite IHts -(mem_undup (b :: get_bs t)) bnode_memP /==> ->; rewrite mem_undup.
-             case: h e=> //= b.
-             by rewrite -(mem_undup (b :: get_bs t)) bnode_memP /==> ->; rewrite !in_cons IHts mem_undup.
-      Qed.
-
-      Lemma uniq_rdf_graph g : uniq g. Proof. exact: ugraph. Qed.
-      Hint Resolve uniq_rdf_graph.
-
-      Lemma mem_triple_terms_ts t ts: t \in ts -> [&& (subject t) \in (terms_ts ts),
-              ((predicate t) \in (terms_ts ts)) & ((object t) \in terms_ts ts)].
-      Proof. case t=> s p o ? ? /=; elim: ts=> [//|hd tl IHts] /= t_mem.
-             apply /and3P; rewrite !terms_ts_cons !mem_undup; move: t_mem; rewrite !in_cons /terms_triple !mem_cat; case/orP.
-             + by move=> /eqP <-; rewrite !mem_undup !in_cons !eqxx /= !orbT.
-             + by move=> /IHts /and3P[-> -> ->]; rewrite !orbT.
-      Qed.
-
-      Lemma mem_triple_terms t g: t \in g -> [&& (subject t) \in (terms g),
-              ((predicate t) \in (terms g)) & ((object t) \in terms g)].
-      Proof. by rewrite terms_graph; apply mem_triple_terms_ts. Qed.
-
-      Lemma bterms_ts b ts : Bnode b \in (terms_ts ts) -> Bnode b \in (bnodes_ts ts).
-      Proof. by move=> mem_term; rewrite mem_undup mem_filter. Qed.
-
-      Lemma bterms b g: Bnode b \in (terms g) -> Bnode b \in (bnodes g).
-      Proof. by rewrite terms_graph; apply bterms_ts. Qed.
-
-      Lemma triple_case t1 t2: t1 = t2 -> [&& (subject t1) == (subject t2),
-            (predicate t1) == (predicate t2) &
-              (object t1) == (object t2)].
-      Proof. by case t1; case t2=> /= ? ? ? ? ? ? ? ? ? ? [] -> -> ->; rewrite !eqxx. Qed.
-
-      Lemma relabeling_term_inj_terms_ts {B2 : eqType} (mu : B -> B2) ts sx sy :
-        {in get_bts ts &, injective mu} ->
-        sx \in terms_ts ts -> sy \in terms_ts ts ->
-                                relabeling_term mu sx = relabeling_term mu sy ->
-                                sx = sy.
-      Proof. case sx; case sy=> /= // bx b_y mu_inj memx memy.
-             by move=> [->].
-             by move=> [->].
-             by move=> [/mu_inj]-> //; rewrite -!bnode_memP !bterms_ts.
-      Qed.
-
-      Lemma relabeling_term_inj_terms {B2 : eqType} (mu : B -> B2) g sx sy :
-        {in get_b g &, injective mu} ->
-        sx \in terms g -> sy \in terms g ->
-                                relabeling_term mu sx = relabeling_term mu sy ->
-                                sx = sy.
-        Proof. apply relabeling_term_inj_terms_ts. Qed.
-
-      Lemma is_pre_iso_inj_ts {B2: eqType} ts (mu : B -> B2) : ({in get_bts ts &, injective mu}) -> {in ts &, injective (relabeling_triple mu)}.
-      Proof.
-        move=> mu_inj; case=> sx ps ox ? ?; case=> sy py oy ? ? /= /mem_triple_terms_ts /= /and3P[memsx mempx memox] /mem_triple_terms_ts /= /and3P[memsy mempy memoy] [] eqs eqp eqo.
-          by apply triple_inj=> /=; apply (relabeling_term_inj_terms_ts mu_inj)=> //.
-      Qed.
-
-      Lemma is_pre_iso_inj_g {B2: eqType} g (mu : B -> B2) : ({in get_b g &, injective mu}) -> {in g &, injective (relabeling_triple mu)}.
-      Proof.
-        move=> mu_inj; case=> sx ps ox ? ?; case=> sy py oy ? ? /= /mem_triple_terms /= /and3P[memsx mempx memox] /mem_triple_terms /= /and3P[memsy mempy memoy] [] eqs eqp eqo.
-          by apply triple_inj=> /=; apply (relabeling_term_inj_terms mu_inj)=> //.
-      Qed.
-
-      Lemma eq_relabeling_triple (i l B1 B2 : eqType) (mu nu : B1 -> B2) : mu =1 nu -> (@relabeling_triple i l _ _ mu) =1 (relabeling_triple nu).
-      Proof. by move=> feq [[]? []? []? ? ?]; apply /triple_inj=> //=; rewrite feq. Qed.
-
-      Lemma eq_relabeling_seq_triple (B1 B2 : eqType) (mu nu : B1 -> B2) : mu =1 nu -> (relabeling_seq_triple mu) =1 (relabeling_seq_triple nu).
-      Proof. by move=> feq; elim=> [//| h t IHtl]; rewrite /= (eq_relabeling_triple feq) IHtl. Qed.
-
-      Lemma perm_eq_relab_uniq g1 g2 mu : perm_eq (relabeling_seq_triple mu g1) g2 -> perm_eq (relabeling_seq_triple mu g1) g2 /\ uniq (relabeling_seq_triple mu g1).
-      Proof. by move=> peq; rewrite (perm_uniq peq) peq. Qed.
-
-      Lemma map_comp_in_id g (mu nu: B -> B) : [seq (nu \o mu) i | i <- get_b g] = get_b g ->
-                                              {in (get_b g), nu \o mu =1 id}.
-      Proof. elim: (get_b g)=> [| h t IHtl]; first by move=> _ x; rewrite in_nil //.
-             move=> [heq teq] x; rewrite in_cons; case e: (x == h)=> /=.
-             + by move: e=> /eqP ->; rewrite heq.
-             + apply IHtl; apply teq.
-      Qed.
-
-      Lemma bterm_eq_mem_get_bs (b: B) ts :
-        (@Bnode I B L b) \in terms_ts ts ->
-                             b \in get_bs (bnodes_ts ts).
-      Proof. by move=> /bterms_ts; rewrite {1}bnodes_map_get_bs (mem_map  (@bnode_inj I B L)). Qed.
-
-      Lemma bterm_eq_mem_get_bts (b: B) ts :
-        (@Bnode I B L b) \in terms_ts ts ->
-                             b \in get_bs (bnodes_ts ts).
-      Proof. by apply bterm_eq_mem_get_bs. Qed.
-
-      Lemma bterm_eq_mem_get_b (b: B) g :
-        (@Bnode I B L b) \in terms g ->
-                             b \in get_b g.
-      Proof. by rewrite terms_graph/get_b; apply bterm_eq_mem_get_bs. Qed.
-
-      Lemma mem_ts_mem_triple_bs t ts b : t \in ts -> Bnode b \in bnodes_triple t -> b \in get_bs (bnodes_ts ts).
-      Proof. move=> /mem_triple_terms_ts; case t=> [[]]s []p []o ? ? //= /and3P[sint pint oint];
-                                              rewrite /bnodes_triple filter_undup mem_undup ?in_cons in_nil // Bool.orb_false_r=> /eqP[eq]; move: sint oint; rewrite ?eq=> sint oint; rewrite bterm_eq_mem_get_bs //.
-             by move: eq=> /eqP; case/orP=> /eqP[->].
-      Qed.
-
-      Lemma mem_ts_mem_triple_bts t ts b : t \in ts -> Bnode b \in bnodes_triple t -> b \in get_bts ts.
-      Proof. by apply mem_ts_mem_triple_bs. Qed.
-
-      Lemma mem_g_mem_triple_b t g b : t \in g -> Bnode b \in bnodes_triple t -> b \in get_b g.
-      Proof. by apply mem_ts_mem_triple_bs. Qed.
-
-      Lemma can_bs_can_rtbs ts (mu nu: B -> B) : {in get_bs (bnodes_ts ts), nu \o mu =1 id} ->
-                                             {in ts, [eta relabeling_triple (nu \o mu)] =1 id}.
-      Proof. move=> /= in_getb [s p o sib pii] /mem_ts_mem_triple_bs ing /=; apply triple_inj=> /=.
-             + case: s sib ing  => // b sib ing.
-               by rewrite /= in_getb // ing // /bnodes_triple filter_undup mem_undup in_cons eqxx.
-             + by case: p pii ing  => // b sib /mem_g_mem_triple_b inb /=.
-             + case: o ing  => // b ing /=.
-               by rewrite /= in_getb // ing // /bnodes_triple filter_undup mem_undup mem_filter -mem_rev in_cons eqxx.
-      Qed.
-
-      Lemma can_bts_can_rtbs ts (mu nu: B -> B) : {in get_bts ts, nu \o mu =1 id} ->
-                                             {in ts, [eta relabeling_triple (nu \o mu)] =1 id}.
-      Proof. by apply can_bs_can_rtbs. Qed.
-
-      Lemma can_b_can_rtb g (mu nu: B -> B) : {in get_b g, nu \o mu =1 id} ->
-                            {in g, [eta relabeling_triple (nu \o mu)] =1 id}.
-      Proof. by apply can_bs_can_rtbs. Qed.
 
       Definition iso_sym g1 g2 : iso g1 g2 <-> iso g2 g1.
       Proof.
@@ -847,26 +799,6 @@ Section Rdf.
         move: perm_relab; rewrite perm_sym=> /(perm_map (relabeling_triple nu))=> perm_relab.
         apply: perm_trans perm_relab _; rewrite relabeling_triple_map_comp map_id_in //.
       Qed.
-
-      Lemma relabeling_triple_comp_map (B1 B2 B3 : eqType) (g : rdf_graph I B1 L) (mu12 : B1 -> B2) (mu23 : B2 -> B3) :
-        [seq relabeling_triple mu23 i | i <- relabeling_seq_triple mu12 g] =
-          relabeling_seq_triple (mu23 \o mu12) g.
-      Proof. case g=> g' us=> /=; rewrite -map_comp.
-             by elim g'=> [//| h t IHts] /=; last by rewrite relabeling_triple_comp -IHts.
-      Qed.
-
-      Lemma perm_eq_comp ts1 ts2 ts3 mu12 mu23:
-        perm_eq (relabeling_seq_triple mu12 ts1) ts2 ->
-        perm_eq (relabeling_seq_triple mu23 ts2) ts3 ->
-        perm_eq (relabeling_seq_triple (mu23 \o mu12) ts1) ts3.
-      Proof. by move=> /(perm_map (relabeling_triple mu23)); rewrite relabeling_triple_map_comp; apply perm_trans. Qed.
-
-      Lemma eqb_relabeling_comp g1 g2 g3 mu12 mu23:
-        forall u1 u2 u3,
-          eqb_rdf (@relabeling _ _ mu12 g1 u1) g2 ->
-          eqb_rdf (@relabeling _ _ mu23 g2 u2) g3 ->
-          eqb_rdf (@relabeling _ _ (mu23 \o mu12) g1 u3) g3.
-      Proof. by move=> u1 u2 u3; apply perm_eq_comp. Qed.
 
       Definition iso_trans g1 g2 g3 : iso g1 g2 -> iso g2 g3 -> iso g1 g3.
       Proof. rewrite /iso/is_iso; move=> [mu12 /and3P[pre_iso12 urel12 perm12]] [mu23 /and3P[pre_iso23 urel23 perm23]].
@@ -882,50 +814,48 @@ Section Rdf.
                by apply eq_mem_map; apply perm_mem.
       Qed.
 
-      Lemma uniq_relabeling_pre_iso mu (ts : seq (triple I B L)):
-        uniq ts -> is_pre_iso_ts ts (relabeling_seq_triple mu ts) mu -> uniq (relabeling_seq_triple mu ts).
-      Proof. by rewrite /is_pre_iso_ts=> uts /is_pre_iso_ts_inj/is_pre_iso_inj_ts ?; rewrite map_inj_in_uniq //. Qed.
-
       Lemma ts_pre_iso_iso ts mu (urel: uniq (relabeling_seq_triple mu ts)) :
         is_pre_iso_ts ts (relabeling_seq_triple mu ts) mu -> is_iso_ts ts (relabeling_seq_triple mu ts) mu.
-      Proof. move=> pre_iso; rewrite /is_iso/is_iso_ts pre_iso urel /=; apply perm_refl. Qed.
+      Proof. by move=> pre_iso; rewrite /is_iso/is_iso_ts pre_iso urel /=; apply perm_refl. Qed.
 
-      Definition isocanonical_mapping (M : rdf_graph I B L -> rdf_graph I B L) :=
-        forall g, iso (M g) g /\
-               (forall g1 g2, eqb_rdf (M g1) (M g2) <-> iso g1 g2).
+      Section Isocanonical.
 
-      Definition mapping_is_iso_mapping (M : rdf_graph I B L -> rdf_graph I B L) := forall g, iso (M g) g.
+        Definition isocanonical_mapping (M : rdf_graph I B L -> rdf_graph I B L) :=
+          forall g, iso (M g) g /\
+                 (forall g1 g2, eqb_rdf (M g1) (M g2) <-> iso g1 g2).
 
-      Definition dt_names_mapping (M : rdf_graph I B L -> rdf_graph I B L) := forall g1 g2,
-          iso g1 g2 -> eqb_rdf (M g1) (M g2).
+        Definition mapping_is_iso_mapping (M : rdf_graph I B L -> rdf_graph I B L) := forall g, iso (M g) g.
 
-      (* forall g μ, {in (get_b g), bijective μ} -> M g == M (relabeling μ g). *)
+        Definition dt_names_mapping (M : rdf_graph I B L -> rdf_graph I B L) := forall g1 g2,
+            iso g1 g2 -> eqb_rdf (M g1) (M g2).
 
-      (* Definition dont_manipulate_names_mapping_idem (M : rdf_graph I B L -> rdf_graph I B L) (dnmn : dont_manipulate_names_mapping M) : forall g (μ : B -> B), (bijective μ) -> M (M g) = M g. *)
+        (* forall g μ, {in (get_b g), bijective μ} -> M g == M (relabeling μ g). *)
 
-      (* Lemma iso_leads_canonical_mapping M (nmn : dt_names_mapping M) g1 g2 : *)
-      (*   iso_mapping g1 g2 -> eqb_rdf (M g1) (M g2). *)
-      (* Proof. rewrite /iso_mapping/is_iso_mapping; move=> [μ /andP [peq eqb]]. *)
-      (*        suffices -> : M g2 = M (relabeling μ g2). by []. *)
-      (*        apply /eqP; apply (nmn g2 μ bijmu). *)
-      (* Qed. *)
+        (* Definition dont_manipulate_names_mapping_idem (M : rdf_graph I B L -> rdf_graph I B L) (dnmn : dont_manipulate_names_mapping M) : forall g (μ : B -> B), (bijective μ) -> M (M g) = M g. *)
 
-      Lemma same_res_impl_iso_mapping M g1 g2 (iso_output : mapping_is_iso_mapping M) : eqb_rdf (M g1) (M g2) -> iso g1 g2.
-      Proof.
-        have isog1k1 : iso g1 (M g1). by rewrite iso_sym; apply iso_output.
-        have isog2k2 : iso (M g2) g2. by apply iso_output.
-        by move=> /eqiso peqm; apply: iso_trans (iso_trans isog1k1 peqm) isog2k2.
-      Qed.
+        (* Lemma iso_leads_canonical_mapping M (nmn : dt_names_mapping M) g1 g2 : *)
+        (*   iso_mapping g1 g2 -> eqb_rdf (M g1) (M g2). *)
+        (* Proof. rewrite /iso_mapping/is_iso_mapping; move=> [μ /andP [peq eqb]]. *)
+        (*        suffices -> : M g2 = M (relabeling μ g2). by []. *)
+        (*        apply /eqP; apply (nmn g2 μ bijmu). *)
+        (* Qed. *)
 
-      Lemma isocanonical_mapping_dt_out_mapping M (iso_out: mapping_is_iso_mapping M) (dt: dt_names_mapping M) : isocanonical_mapping M.
-      Proof.
-        split; first by apply iso_out.
-        split; last by apply dt.
-        + by apply: same_res_impl_iso_mapping iso_out.
-      Qed.
+        Lemma same_res_impl_iso_mapping M g1 g2 (iso_output : mapping_is_iso_mapping M) : eqb_rdf (M g1) (M g2) -> iso g1 g2.
+        Proof.
+          have isog1k1 : iso g1 (M g1). by rewrite iso_sym; apply iso_output.
+          have isog2k2 : iso (M g2) g2. by apply iso_output.
+          by move=> /eqiso peqm; apply: iso_trans (iso_trans isog1k1 peqm) isog2k2.
+        Qed.
+
+        Lemma isocanonical_mapping_dt_out_mapping M (iso_out: mapping_is_iso_mapping M) (dt: dt_names_mapping M) : isocanonical_mapping M.
+        Proof.
+          split; first by apply iso_out.
+          split; last by apply dt.
+          + by apply: same_res_impl_iso_mapping iso_out.
+        Qed.
 
 
-
+      End Isocanonical.
     End Isomorphism.
 
   End EqRdf.
